Since 
\begin{align}\label{ec/2021/41/Z1}
a^nu(-n-1) &\zed \frac{1}{1-az^{-1}}  \quad \abs{z} < \abs{a},
\\
X(z) &=  \frac{4z^{-3}}{1-2z^{-1}}  \quad \abs{z} < 2,
\\
Y(z) &= \frac{8z}{1-\frac{1}{2}z^{-1}}  \quad \abs{z} > \frac{1}{2}
    \end{align}
and     
\begin{align}\label{ec/2021/41/Zf}
x(n)*y(-n) &\zed \frac{32z^{-4}}{\brak{1-2z^{-1}}\brak{1-\frac{1}{2}z}} \quad  \abs{z} < 2,
\\
\implies z(n) &= x(n)*y(-n) =  (4-n)2^{n+1}u[4-n]
        \end{align}
\begin{align}
    \therefore \frac{1}{2\pi} \int_{0}^{2\pi} X(e^{j\omega}) Y(e^{-j\omega}) \, d\omega =z[0]=8
\end{align}
