
\begin{definition}[Dirac-delta impulse]
\begin{align}
 \delta\brak{t}=
 \begin{cases}
 \infty , & t=0\\
 0, & otherwise
 \end{cases}
\end{align}
\end{definition}
\begin{lemma}[Shifting property of $\delta\brak{t}$]
 If $g\brak{t}$ is a continuous and finite function at $t=a$ then
 \begin{align}
     \int_{-\infty}^{\infty}\delta\brak{t-a}g\brak{t}dt=g\brak{a}
 \end{align}
 We also have
 \begin{align}
     \int_{-\infty}^{\infty}\delta\brak{t-a}\delta\brak{t-b}dt=\delta\brak{a-b}\label{translation}
 \end{align}
\end{lemma}
%%%%%%%%%
\begin{theorem}
Fourier transform of shifted impulse is the complex exponential.
\begin{align}
    G\brak{f}=\mathcal{F}\cbrak{\delta\brak{t-a}}=e^{-i2\pi fa}
\end{align}
\end{theorem}
\begin{proof}
 \begin{align}
     G\brak{f}&=\int_{-\infty}^{\infty}\delta\brak{t-a}e^{-i2\pi ft}dt\\
     &=e^{-i2\pi fa}
 \end{align}
\end{proof}
%%%%%%%%%
\begin{corollary}
Inverse Fourier Transform of the complex exponential must be the shifted impulse. So
\begin{align}
    \mathcal{F}^{-1}\cbrak{e^{-2\pi fa}}&=\int_{-\infty}^{\infty}e^{-2\pi fa}e^{i2\pi ft}df\\
    &=\int_{-\infty}^{\infty}e^{i2\pi f\brak{t-a}}df\\
    &=\int_{-\infty}^{\infty}e^{-i2\pi f\brak{t-a}}df\\
    &=\delta\brak{t-a}
\end{align}
\end{corollary}
%%%%%%%%%
\begin{theorem}
The Fourier transform of $g\brak{t}=e^{i2\pi at}$ is given by 
\begin{align}
    G\brak{f}=\mathcal{F}\cbrak{e^{i2\pi at}}=\delta\brak{f-a}
\end{align}
\begin{proof}
 \begin{align}
     G\brak{f}&=\int_{-\infty}^{\infty}e^{i2\pi at}e^{-i2\pi ft}dt\\
     &=\int_{-\infty}^{\infty}e^{i2\pi t\brak{a-f}}dt\\
     &=\delta\brak{f-a}
 \end{align}
\end{proof}
\end{theorem}
%%%%%%%%
\begin{lemma}[Linearity of Fourier Transform]
\begin{align}
    \mathcal{F}\cbrak{c_1g\brak{t}+c_2h\brak{t}}=c_1\mathcal{F}\cbrak{g\brak{t}}+c_2\mathcal{F}\cbrak{h\brak{t}}
\end{align}
\end{lemma}
%%%%%%%
\begin{lemma}\label{fre}
Let $x\brak{t}$ be a signal, its Fourier Transform  be of the form
\begin{align}
    G_x\brak{f}=c_1\delta\brak{f-a_1A}+c_2\delta\brak{f-a_2A}+...
\end{align}
where $c_i\in \mathbb{C}$ and $a_i\in \mathbb{R}$. 
Then the frequencies present in the signal are $a_jA $ where $a_j\in \mathbb{R}^{+}$
\end{lemma}
%%%%%%%
Let $x\brak{t}=\cos{\brak{2\pi At}}$, where $A=10kHz$.
\begin{align}
  \cos{\brak{2\pi At}}=\frac{e^{i2\pi At}+e^{-i2\pi At}}{2}  
\end{align}
The Fourier transform of $x\brak{t}$ 
\begin{align}
    G_x\brak{f}&=\int_{-\infty}^{\infty}\frac{e^{i2\pi At}+e^{-i2\pi At}}{2}e^{-i2\pi ft}dt\\
    &=\frac{1}{2}\sbrak{\int_{-\infty}^{\infty}e^{-i2\pi t(f-A)}dt+\int_{-\infty}^{\infty}e^{-i2\pi t(A+F)}}\\
    &=\frac{1}{2}\sbrak{\delta\brak{f-A}+\delta\brak{f+A}}
\end{align}
$\therefore$ All the energy of the sinusoidal wave is  entirely localized at the frequencies given by $|f|=A$.
\begin{align}
    y\brak{t}&=\cos{\brak{2\pi At}}\cos{\brak{2\pi A\brak{1+\frac{t}{2}}}}\\
    &=\frac{1}{2}\brak{\cos{\brak{2\pi A+3\pi At}}+\cos{\brak{2\pi A-\pi At}}}\\
    &=\frac{1}{2}\brak{\cos{\brak{3\pi At}}+\cos{\brak{\pi At}}\label{yt}}
\end{align}
Fourier Transform of $y\brak{t}$ is given by
\begin{multline}
    G_y\brak{f}=\frac{1}{4}\sbrak{\delta\brak{f-\frac{3A}{2}}+\delta\brak{f+\frac{3A}{2}}}\\+\frac{1}{4}\sbrak{\delta\brak{f-\frac{A}{2}}+\delta\brak{f+\frac{A}{2}}}
\end{multline}
From lemma $\ref{fre}$ we can conclude that the frequencies present in signal $y\brak{t}$ are $\frac{A}{2},\frac{3A}{2}$
\begin{lemma}{Multiplication property of Fourier Transform}\label{conv}
\begin{align}
    \text{If } x\brak{t} \fourier X\brak{f} \\
    y\brak{t} \fourier Y\brak{f}
\end{align}
Then
\begin{align}
   x\brak{t}y\brak{t} \fourier  X\brak{f} \ast Y\brak{f}
\end{align}
where $\ast$ represents convolution
\end{lemma}
\begin{lemma}
\begin{align}
    \delta\brak{t-t_0}\ast g\brak{t}=g\brak{t-t_0}\label{convdelta}
\end{align}
\end{lemma}
\begin{lemma}{Computing $G_y\brak{f}$ using convolution}
\begin{align}
    x\brak{t}&=\cos{\brak{2\pi At}}\\
    x\brak{t}& \fourier X_1\brak{f}=\frac{1}{2}\sbrak{\delta\brak{f-A}+\delta\brak{f+A}}\\
    x\brak{1+\frac{t}{2}}&=\cos{\brak{\pi At}}\\
    x\brak{1+\frac{t}{2}}& \fourier X_2\brak{f}=\frac{1}{2}\sbrak{\delta\brak{f-\frac{A}{2}}+\delta\brak{f+\frac{A}{2}}}
\end{align}
Using lemma $\ref{conv}$ 
\begin{align}
    G_y\brak{f}&=X_1\brak{f}\ast X_2\brak{f}\\
    &=\brak{\frac{1}{2}\sbrak{\delta\brak{f-A}+\delta\brak{f+A}}}\ast  X_2\brak{f}\\
    &=\frac{1}{2}\cbrak{\delta\brak{f-A}\ast  X_2\brak{f}+\delta\brak{f+A}\ast  X_2\brak{f}}
\end{align}
Using $\eqref{convdelta}$ 
\begin{align}
    G_y\brak{f}=\frac{1}{2}\brak{X_2\brak{f-A}+X_2\brak{f+A}}
\end{align}
\begin{multline}
    G_y\brak{f}=\frac{1}{4}\sbrak{\delta\brak{f-\frac{3A}{2}}+\delta\brak{f+\frac{3A}{2}}}\\+\frac{1}{4}\sbrak{\delta\brak{f-\frac{A}{2}}+\delta\brak{f+\frac{A}{2}}}
\end{multline}
\end{lemma}
\begin{align}
  x\brak{t}&=\cos{\brak{20k\pi t}}\\
    \text{bandwidth of } x\brak{t} &= 10 kHz\\
    x\brak{1+\frac{t}{2}} &= \cos{\brak{20k\pi+10k\pi t}}\\
    \text{bandwidth of } x\brak{1+\frac{t}{2}} &=  5 kHz\\
    \text{from \eqref{yt} } 
    y\brak{t}&= \cos{\brak{30k\pi t}}+\cos{\brak{10k\pi t}}\\
    \text{bandwidth of } y\brak{t} &= \frac{30}{2} kHz\\
    &= 15 kHz
\end{align}
\begin{align}
    \text{Nyquist rate} &= 2 \times \text{maximum frequency}\\
    &= 30 kHz
\end{align}
\begin{figure}[!h]
 \centering
 \includegraphics[width=\columnwidth]{solutions/ec/2021/4/figs/x.png}
 \caption{$x\brak{t}$:Sinusoidal signal with freq=10kHz}
\end{figure}
\begin{figure}[!h]
 \centering
 \includegraphics[width=\columnwidth]{solutions/ec/2021/4/figs/xf.png}
 \caption{DFT of $x\brak{t}$. $Bandwidth=10000$}
\end{figure}
\begin{figure}[!h]
 \centering
 \includegraphics[width=\columnwidth]{solutions/ec/2021/4/figs/four_y.png}
 \caption{DFT of $y\brak{t}$.$Bandwidth=15000$}
\end{figure}
\begin{figure}[!h]
 \centering
 \includegraphics[width=\columnwidth]{solutions/ec/2021/4/figs/stem_y.png}
 \caption{stem plot of $y\brak{t}$ sampled at 60kHz}
\end{figure}
\begin{figure}[!h]
 \centering
 \includegraphics[width=\columnwidth]{solutions/ec/2021/4/figs/interpolation.png}
 \caption{Shannon interpolation of $y\brak{t}$}
\end{figure}


